Veritas.Verifier.Merkle.fsti
@@ -2,6 +2,7 @@ module Veritas.Verifier.Merkle
 
 open FStar.Seq
 open Veritas.BinTree
+open Veritas.EAC
 open Veritas.Hash
 open Veritas.Key
 open Veritas.Record
@@ -9,6 +10,7 @@ open Veritas.SeqAux
 open Veritas.Verifier
 open Veritas.Verifier.TSLog
 
+module E=Veritas.EAC
 module I = Veritas.Interleave
 module V = Veritas.Verifier
 module TL = Veritas.Verifier.TSLog
@@ -70,6 +72,17 @@ val lemma_addm_ancestor_is_proving (itsl: its_log {I.length itsl > 0}):
                   let itsl' = I.prefix itsl (n - 1) in
                   let k = V.key_of e in
                   Root <> k /\ AddM?.k' e = proving_ancestor itsl' k))
+
+let is_in_blum (es: E.eac_state): bool = 
+  EACEvictedBlum? es || 
+  (EACInStore? es && EACInStore?.m es = BAdd)
+
+let proving_ancestor_has_blum_bit (itsl: TL.eac_log) (k:key {k <> Root}): bool = 
+  let es = TL.eac_state_of_key itsl k in
+  not (E.is_eac_state_active es) || 
+  mv_evicted_to_blum (eac_merkle_value itsl (proving_ancestor itsl k))
+                                     (desc_dir k (proving_ancestor itsl k)) =
+                      is_in_blum es
 
 (* when evicted as blum the proving ancestor contains a bit indicating the eviction *)
 val lemma_proving_ancestor_blum_bit (itsl: TL.eac_log) (k:key{k <> Root}):
